TEEE.v
@@ -1,0 +1,76 @@
+Inductive Types :=
+ | rpms
+ | meterscubedpersecond
+ | volts
+ | degreesC
+ | function
+ | millimeters
+ | boolstate
+ . 
+ 
+Inductive VarIdentifier :=
+ | vnat : nat -> VarIdentifier
+ | vReturn. 
+ 
+Inductive TypedVar : Types -> Set  :=
+ | VarRPMs : VarIdentifier -> nat -> TypedVar rpms.  
+
+
+Inductive Measurement : Type := 
+ | MotorSpeed
+ | MotorInterpolation
+ | BatteryVoltage_
+ | BriefDischargeTest
+ | Temperature_
+ | TubeDiameter
+ | MotorOn.
+
+Inductive InterpolationMethod :Set :=
+ | Linear
+ | Quadratic.
+
+Definition measurementTypes (m : Measurement) : Types :=
+match m with
+ | MotorSpeed => rpms
+ | BatteryVoltage_ => volts
+ | BriefDischargeTest => volts
+ | Temperature_ => degreesC
+ | TubeDiameter => millimeters
+ | MotorOn => boolstate
+ | MotorInterpolation => function
+end.
+
+Definition TypesDenote (t : Types) :=
+match t with
+ | rpms => nat
+ | meterscubedpersecond => nat
+ | volts => nat
+ | degreesC => nat
+ | function => nat -> nat
+ | millimeters => nat
+ | boolstate => bool
+end. 
+Eval compute in (TypesDenote function).
+
+ 
+Definition measure (m : Measurement) : (TypesDenote (measurementTypes m)).
+Admitted.   
+
+Definition Time := nat. 
+(* The calculation language *)
+Inductive Calculation :=
+ | calcMeasure (m : Measurement) : 
+     Time ->  TypedVar (measurementTypes m) -> Calculation 
+ | calcDelay : 
+     Calculation -> nat -> Calculation. 
+     
+Inductive Var :=
+ | var : forall t : Types,  TypedVar t -> Var. 
+
+Inductive Program :=
+ | Calc : Var ->  Calculation -> Program
+ | Measure (m : Measurement) :
+     TypedVar (measurementTypes m) -> 
+ | Delay : nat -> Program
+ | Chain : Program -> Program -> Program.
+ 
